Core/Metatheory/Progress.lean
@@ -1,6 +1,7 @@
 import Core.Term
 import Core.Reduction
 import Core.Typing
+import Core.Metatheory.Closed
 
 open Lilac
 open LeanSubst
@@ -10,13 +11,37 @@ namespace Core
 @[grind →]
 theorem spctor_inversion :
   ¬ v = .openm ->
-  G&Δ,Γ ⊢ Term.spctor v s tys ts : T ->
+  G&Δ,Γ ⊢ Term.spctor v s As Bs ts : T ->
   T.spine.isSome
 := by
   intro j1 j2
-  cases j2; case _ j2 j3 j4 j5 j6 j7 j8 =>
+  cases j2; case _ j2 j3 j4 j5 j6 j7 j8 j9 =>
   cases v <;> simp at j1; case _ c =>
-  replace j4 := j4 c rfl; subst j8
+  -- replace j4 := j4 c rfl; subst j8
+  sorry
+
+theorem lookup_ctor?_subst (σ : Subst Ty) : lookup_ctor? G c x R -> lookup_ctor? G c x R[σ] := by
+  intro h; unfold lookup_ctor? at *
+  generalize zdef : R.spine = z at *
+  cases z <;> simp at h; case _ z =>
+  rcases z with ⟨z, sp⟩; simp at h
+  have lem : R[σ].spine = some (z, sp[σ]) := sorry
+  rw [lem]; simp [*]
+
+theorem lookup_ctor?_data?_force_dataconst (σ : Subst Ty) :
+  lookup_ctor? G v1 x R ->
+  Ty.data? v2 G R[σ] = true ->
+  v2 = v1
+:= by
+  intro h1 h2
+  unfold lookup_ctor? at h1
+  unfold Ty.data? at h2
+  generalize zdef : R.spine = z at *
+  cases z; simp at *; case _ z =>
+  rcases z with ⟨z, sp⟩; simp at *
+  have lem : R[σ].spine = some (z, sp[σ]) := sorry
+  rw [lem] at h2; simp at h2
+  unfold is_data at h2
   sorry
 
 theorem split_all_or_left : ∀ {n} {A B : Fin n -> Prop}, (∀ i, A i ∨ B i) -> (∀ i, A i) ∨ (∃ i, B i)
@@ -32,15 +57,12 @@ theorem split_all_or_left : ∀ {n} {A B : Fin n -> Prop}, (∀ i, A i ∨ B i) 
   | Or.inr ⟨k, lem'⟩ => Or.inr ⟨k.succ, lem'⟩
 
 theorem PatternBinders.implies_pattern_typing :
-  PatternBinders G Δ m S p ξ ->
+  PatternBinders G Δ m S p ζ ξ ->
   PatternTyping G Δ p S
-| .zero => by
-  rw [Vec.nil_singleton S .nil]
-  rw [Vec.nil_singleton p .nil]
-  exact VecTyping.nil
+| .zero => by cases S; cases p; apply VecTyping.nil
 | .succ h1 h2 h3 h4 h5 tl =>
   let tl' := tl.implies_pattern_typing
-  let lem := .valid h1 h3 h2 h5
+  let lem := .valid h1 h2 h5
   .cons lem tl'
 
 @[simp]
@@ -63,27 +85,28 @@ theorem progress_match_ctors_head {ctors : Vec _ n} :
   G&Δ,Γ ⊢ s : S ->
   Ty.data? cv G S ->
   Value G s ->
-  VecConstructorTyping G Δ Γ ctors SS ->
+  VecConstructorTyping G Δ Γ cv ctors SS ->
   Term.IsData cv ss ctors ->
   Query G cv (Constructor.query ctors) SS ->
-  ∃ ctors, VecConstructorTyping G Δ Γ ctors (S::SS)
+  ∃ ctors, VecConstructorTyping G Δ Γ cv ctors (S::SS)
     ∧ Term.IsData cv (s::ss) ctors
     ∧ Query G cv (Constructor.query ctors) (S::SS)
-| .spctor (x := x) (v := .data cv') (m := na) (As := As) (n := nt) (ts := ts) j1 j2 j3 j4 j5 j6 j7
-  , h2, .spctor h, h4, h5, h6 =>
-  have lem1 : cv = cv' := sorry
-  let ctors' := ⟨x, na, As, nt, ts.to⟩::ctors
-  let lem2hd : ConstructorTyping G Δ Γ (x, ⟨na, (As, ⟨nt, ts.to⟩)⟩) S :=
-    .valid j1 j2 j3 (j4 |> cast (by simp)) j7
-  let lem2 : VecConstructorTyping G Δ Γ ctors' (S :: SS) := VecTyping.cons lem2hd h4
-  let lem3 : Term.IsData cv (.spctor (.data cv') x As ts::ss) ctors' :=
+| .spctor (v := .data cv') (x := x) (m1 := na) (As := As) (m2 := nb) (Bs := Bs) (n := nt) (ts := ts) j1 j2 j3 j4 j5 j6 j7 j8 j9
+, h2, .spctor h, h4, h5, h6 =>
+  have lem1 : cv = cv' := lookup_ctor?_data?_force_dataconst
+    (List.map su (As.list ++ Bs.list).reverse ++ Subst.id Ty) (j7 _ rfl) (by subst j3; apply h2)
+  let ctors' := ⟨x, na, As, nb, Bs, nt, ts.to⟩::ctors
+  have lem2hd : ConstructorTyping G Δ Γ cv ⟨x, na, As, nb, Bs, nt, ts.to⟩ S :=
+    .valid (x := x) j1 (j7 cv' rfl |> cast (by simp [lem1])) j2 j3 (j4 |> cast (by simp)) j5 (j6 |> cast (by simp [Vec.get_to]))
+  have lem2 : VecConstructorTyping G Δ Γ cv ctors' (S :: SS) := VecTyping.cons lem2hd h4
+  have lem3 : Term.IsData cv (.spctor (.data cv') x As Bs ts::ss) ctors' :=
     Term.IsData.cons h5 (by simp [lem1]) rfl
-  let lem4 : Query G cv (Constructor.query ctors') (S::SS) :=
-    VecTyping.cons (by simp; sorry) h6
+  have lem4 : Query G cv (Constructor.query ctors') (S::SS) :=
+    VecTyping.cons (by simp; subst j3; rw [lem1]; apply lookup_ctor?_subst _ (j7 _ rfl)) h6
   ⟨ctors', lem2, lem3, lem4⟩
-| .refl j, h2, .refl, h4, h5, h6 => by simp [Ty.data?, Ty.HeadVariable, Ty.spine] at h2
-| .lam j1 j2, h2, .lam, h4, h5, h6 => by simp [Ty.data?, Ty.HeadVariable, Ty.spine] at h2
-| .lamt j1 j2, h2, .lamt, h4, h5, h6 => by simp [Ty.data?, Ty.HeadVariable, Ty.spine] at h2
+| .refl j, h2, .refl, h4, h5, h6 => by simp [Ty.data?, Ty.spine] at h2
+| .lam j1 j2, h2, .lam, h4, h5, h6 => by simp [Ty.data?, Ty.spine] at h2
+| .lamt j1 j2, h2, .lamt, h4, h5, h6 => by simp [Ty.data?, Ty.spine] at h2
 
 theorem progress_match_ctors :
   {m : Nat} ->
@@ -91,7 +114,7 @@ theorem progress_match_ctors :
   (∀ (i : Fin m), G&Δ,Γ ⊢ ss[i] : S[i]) ->
   (∀ (i : Fin m), Ty.data? c G S[i]) ->
   (∀ (i : Fin m), Value G ss[i]) ->
-  ∃ ctors, VecConstructorTyping G Δ Γ ctors S
+  ∃ ctors, VecConstructorTyping G Δ Γ c ctors S
     ∧ Term.IsData c ss ctors
     ∧ Query G c (Constructor.query ctors) S
 | 0, .nil, .nil, h1, h2, h3 => ⟨.nil, .nil, Term.IsData.nil, .nil⟩
@@ -103,7 +126,7 @@ theorem progress_match_ctors :
   progress_match_ctors_head (h1 0) (h2 0) (h3 0) q1 q2 q3
 
 theorem query_match_implies_pattern_match (G : List Global) {n : Nat} {c q p Ts : Vec _ n} :
-  VecConstructorTyping G Δ Γ c Ts ->
+  VecConstructorTyping G Δ Γ v c Ts ->
   PatternTyping G Δ p Ts ->
   Constructor.query c = q ->
   Query.Match q p ->
@@ -115,7 +138,7 @@ theorem query_match_implies_pattern_match (G : List Global) {n : Nat} {c q p Ts 
     injection h1 with he0 he1 he2; clear he0; subst he1 he2
     rcases e1 with ⟨na', As', nb', he0⟩; subst he0
     cases ctj; case _ e1 _ _ =>
-    cases ptj; case _ e2 _ =>
+    cases ptj; case _ e2 _ _ =>
     rw [e2] at e1
     injection e1 with e1
     cases e1
@@ -129,44 +152,53 @@ theorem progress (oe : OpenExhaustive G) :
   Γ = [] ->
   Value G t ∨ ∃ t', G ⊢ t ~> t'
 | .defn j1 j2, e => Or.inr ⟨_, .defn j1⟩
-| .spctor (v := .data .cls) j1 j2 j3 j4 j5 j6 j7, e => Or.inl $ Value.spctor (by simp)
-| .spctor (v := .data .opn) j1 j2 j3 j4 j5 j6 j7, e => Or.inl $ Value.spctor (by simp)
-| @Typing.spctor G m n x Ks Ts R Δ τ Γ .openm R' As ts j1 j2 j3 j4 j5 j6 j7, e =>
-  let j4' := λ i => progress oe (j4 i) e
-  match split_all_or_left j4' with
+| .spctor (v := .data .cls) j1 j2 j3 j4 j5 j6 j7 j j9, e => Or.inl $ Value.spctor (by simp)
+| .spctor (v := .data .opn) j1 j2 j3 j4 j5 j6 j7 j8 j9, e => Or.inl $ Value.spctor (by simp)
+| @Typing.spctor G Δ Γ m1 m2 n x .openm Ks1 Ks2 Ts Ts' R R' As Bs ts j1 j2 j3 j4 j5 j6 j7 j8 j9, e =>
+  let j6' := λ i => progress oe (j6 i) e
+  match split_all_or_left j6' with
   | Or.inl vs =>
-    let Ts' : Vec Ty n := Vec.map (·[τ]) Ts
-    let j1' : ∀ (i : Fin n), G&Δ,Γ ⊢ ts.to[i] : Ts'[i] := j4 |> cast (by subst Ts'; simp)
-    let j2' : ∀ (i : Fin n), Ty.data? .opn G Ts'[i] := (j6 rfl) |> cast (by subst Ts'; simp)
-    let vs' : ∀ (i : Fin n), Value G ts.to[i] := vs |> cast (by simp)
-    let ⟨ctors, h1, h2, h3⟩ := progress_match_ctors j1' j2' vs'
-    let lem1 : lookup x G = some (.openm x ⟨m, Ks, n, Ts, R⟩) := sorry
-    let ⟨i, b, p, lem2, lem3⟩ := oe (q := Constructor.query ctors) lem1 j2 j3 (by congr) (h3 |> cast (by congr))
-    let lem4 : PatternTyping G Δ p Ts' := sorry
-    let lem5 := query_match_implies_pattern_match G h1 lem4 rfl lem3
-    let σ := Constructor.subst ctors
-    Or.inr ⟨_, .openm_match (σ := σ) h2 lem2 j3 lem5 rfl⟩
+    sorry
+  --   let Ts' : Vec Ty n := Vec.map (·[τ]) Ts
+  --   let j1' : ∀ (i : Fin n), G&Δ,Γ ⊢ ts.to[i] : Ts'[i] := j4 |> cast (by subst Ts'; simp)
+  --   let j2' : ∀ (i : Fin n), Ty.data? .opn G Ts'[i] := (j6 rfl) |> cast (by subst Ts'; simp)
+  --   let vs' : ∀ (i : Fin n), Value G ts.to[i] := vs |> cast (by simp)
+  --   let ⟨ctors, h1, h2, h3⟩ := progress_match_ctors j1' j2' vs'
+  --   let lem1 : lookup x G = some (.openm x ⟨m, Ks, n, Ts, R⟩) := sorry
+  --   let ⟨i, b, p, lem2, lem3⟩ := oe (q := Constructor.query ctors) lem1 j2 j3 (by congr) (h3 |> cast (by congr))
+  --   let lem4 : PatternTyping G Δ p Ts' := sorry
+  --   let lem5 := query_match_implies_pattern_match G h1 lem4 rfl lem3
+  --   let σ := Constructor.subst ctors
+  --   Or.inr ⟨_, .openm_match (σ := σ) h2 lem2 j3 lem5 rfl⟩
   | Or.inr ⟨i, t', r⟩ =>
-    let ts' := Fun.Vec.update ts t' i
-    let r' : G ⊢ ts i ~> ts' i := by subst ts'; simp; exact r
-    Or.inr ⟨_, .openm_congr i r' Fun.Vec.update_neq⟩
+    let ts' := Vec.set ts.to i t'
+    let r' : G ⊢ ts i ~> ts'[i] := by subst ts'; simp; exact r
+    Or.inr ⟨_, .openm_congr i r' (by {
+      intro j h; simp [ts']
+      have lem := Vec.get_set_neq (Ne.symm h) (v := ts.to) (x := t')
+      rw [Vec.get_to] at lem; rw [<-lem]; simp [getElem]
+    })⟩
 | .mtch (m := m) (S := S) (ss := ss) j1 j2 j3 j4 j5, e =>
   let j1' := λ i => progress oe (j1 i) e
   match split_all_or_left j1' with
   | Or.inl vs =>
-    let j1' : ∀ (i : Fin m), G&Δ,Γ ⊢ ss.to[i] : S.to[i] := j1 |> cast (by simp)
-    let j2' : ∀ (i : Fin m), Ty.data? .cls G S.to[i] := j2 |> cast (by simp)
-    let vs' : ∀ (i : Fin m), Value G ss.to[i] := vs |> cast (by simp)
+    let j1' : ∀ (i : Fin m), G&Δ,Γ ⊢ ss.to[i] : S.to[i] := j1 |> cast (by simp [Vec.get_to])
+    let j2' : ∀ (i : Fin m), Ty.data? .cls G S.to[i] := j2 |> cast (by simp [Vec.get_to])
+    let vs' : ∀ (i : Fin m), Value G ss.to[i] := vs |> cast (by simp [Vec.get_to])
     let ⟨ctors, h1, h2, h3⟩ := progress_match_ctors j1' j2' vs'
     let ⟨i, h4⟩ := j5 h3
     let h5 := PatternBinders.implies_pattern_typing (j3 i)
     let lem1 := query_match_implies_pattern_match G h1 h5 rfl h4
-    let σ := Constructor.subst ctors
-    Or.inr ⟨_, .data_match (σ := σ) h2 lem1 rfl⟩
+    let ℓ := Constructor.subst ctors
+    Or.inr ⟨_, .data_match h2 lem1 rfl⟩
   | Or.inr ⟨i, t', r⟩ =>
-    let ss' := Fun.Vec.update ss t' i
-    let r' : G ⊢ ss i ~> ss' i := by subst ss'; simp; exact r
-    Or.inr ⟨_, .match_congr i r' Fun.Vec.update_neq⟩
+    let ss' := Vec.set ss.to i t'
+    let r' : G ⊢ ss i ~> ss'[i] := by subst ss'; simp; exact r
+    Or.inr ⟨_, .match_congr i r' (by {
+      intro j h; simp [ss']
+      have lem := Vec.get_set_neq (Ne.symm h) (v := ss.to) (x := t')
+      rw [Vec.get_to] at lem; rw [<-lem]; simp [getElem]
+    })⟩
 | .lam j1 j2, e => Or.inl Value.lam
 | .app j1 j2, e =>
   match progress oe j1 e with
