Core/Term/Definition.lean
@@ -11,7 +11,6 @@ inductive DataConst where
 | opn
 | cls
 
-
 inductive Ctor0Variant : Type where
 | refl (A : Ty)
 
