Core/Ty.lean
@@ -2,3 +2,4 @@ import Core.Ty.Definition
 import Core.Ty.BEq
 import Core.Ty.Substitution
 import Core.Ty.Structure
+import Core.Ty.FreeVars
