Core/Ty/FreeVars.lean
@@ -1,0 +1,219 @@
+import LeanSubst
+import Core.Ty.Definition
+import Core.Ty.BEq
+import Core.Ty.Substitution
+
+open LeanSubst
+
+namespace Core
+
+inductive Ty.FV : Ty -> Nat -> Prop where
+| var : FV t#x x
+| arrowr : FV a x -> FV (a -:> b) x
+| arrowl : FV b x -> FV (a -:> b) x
+| eqr : FV a x -> FV (a ~[K]~ b) x
+| eql : FV b x -> FV (a ~[K]~ b) x
+| appr : FV a x -> FV (a • b) x
+| appl : FV b x -> FV (a • b) x
+| all : FV p (a + 1) -> FV (∀[K] p) a
+
+@[simp]
+def Ty.fv : Ty -> Nat -> Bool
+| gt#_, _ => false
+| t#x, i => x == i
+| A -:> B, i => A.fv i || B.fv i
+| A ~[_]~ B, i => A.fv i || B.fv i
+| .app A B, i => A.fv i || B.fv i
+| ∀[_] P, i => P.fv (i + 1)
+
+-- R[ℓ1 ++ σ] = R2[ℓ2 ++ τ] -> ℓ1 = ℓ2
+
+instance instMembership_Nat_Ty : Membership Nat Ty where
+  mem := Ty.FV
+
+theorem Ty.FV.reflection {A : Ty} : i ∈ A <-> A.fv i := by
+  apply Iff.intro <;> intro h
+  case _ => induction h <;> simp [*]
+  case _ =>
+    fun_induction Ty.fv
+    case _ => cases h
+    case _ => simp at h; subst h; apply var
+    case _ ih1 ih2 =>
+      simp at h; cases h
+      case _ h => apply arrowr (ih1 h)
+      case _ h => apply arrowl (ih2 h)
+    case _ ih1 ih2 =>
+      simp at h; cases h
+      case _ h => apply eqr (ih1 h)
+      case _ h => apply eql (ih2 h)
+    case _ ih1 ih2 =>
+      simp at h; cases h
+      case _ h => apply appr (ih1 h)
+      case _ h => apply appl (ih2 h)
+    case _ ih => apply all (ih h)
+
+@[simp]
+def iterate (f : T -> T) : Nat -> T -> T
+| 0 => λ x => x
+| n + 1 => λ x => f $ (iterate f n) x
+
+notation f "^[" n "]" => iterate f n
+
+@[simp]
+theorem iterate_succ {x : Nat} : ((Ren.succ T).act^[n]) x = x + n := by
+  induction n <;> simp at *
+  case succ n ih => rw [ih]; omega
+
+-- theorem lift_iterated_succ_is_re {y : Nat} :
+--   ((Ren.lift^[n]) (Ren.succ Ty)).act y = z ->
+--   ∃ i, z = re i
+-- := by
+--   intro h
+--   induction n generalizing y z <;> simp [-Subst.rewrite_lift_k] at *
+--   case zero => exists y + 1; symm at h; assumption
+--   case succ n ih =>
+--     cases y <;> simp [-Subst.rewrite_lift_k] at *
+--     case zero => exists 0; symm at h; assumption
+--     case succ y =>
+--       sorry
+      -- simp [-Subst.rewrite_lift_k, Subst.compose] at *
+      -- rcases (@ih y) with ⟨k, ih⟩
+      -- generalize zdef : (((Subst.lift (T := Ty))^[n]) +1) y = z at *
+      -- cases z <;> simp [-Subst.rewrite_lift_k] at *
+      -- case _ a =>
+      --   exists (a + 1); symm at h
+      --   rw [zdef] at h; simp [*]
+      -- case _ a =>
+      --   rw [ih] at zdef
+      --   injection zdef
+
+-- x ∉ T[(x + 1)]
+theorem FV.var_not_in_one_more {T : Ty} : (x ∉ T⟨((Ren.lift)^[x]) (Ren.succ Ty)⟩) := by
+  intro h
+  induction T generalizing x <;> simp [-Subst.rewrite_lift_k] at *
+  case var y =>
+    induction x generalizing y <;> simp [-Subst.rewrite_lift_k]  at *
+    case zero => cases h
+    case succ n ih =>
+    cases y <;> simp [-Subst.rewrite_lift_k]  at *
+    case zero => cases h
+    case succ y =>
+    sorry
+    -- simp [Subst.compose] at h
+    -- replace ih := ih y
+    -- generalize zdef : (((Subst.lift (T := Ty))^[n]) +1 y) = z at *
+    -- have lem := lift_iterated_succ_is_re zdef
+    -- rcases lem with ⟨k , lem⟩
+    -- subst z; simp [-Subst.rewrite_lift_k] at lem; rw [lem] at h; simp at h
+    -- cases h; apply ih; rw[lem]; simp; apply Ty.FV.var
+  case all P ih =>
+    cases h; case _ h =>
+    apply @ih (x + 1); simp; apply h
+  case global => cases h
+  all_goals (
+  case _ ih1 ih2 =>
+    replace ih1 := @ih1 x
+    replace ih2 := @ih2 x
+    cases h <;> simp at *
+    case _ h => apply ih1 h
+    case _ h => apply ih2 h)
+
+theorem FV.mem_add {T : Ty} : x ∈ T⟨.add Ty k⟩ -> x ≥ k := by
+  intro h
+  generalize Zdef : T⟨Ren.add Ty k⟩ = Z at *
+  induction h generalizing T k
+  case var =>
+    cases T <;> simp at Zdef
+    subst Zdef; simp
+  case arrowr ih =>
+    cases T <;> simp at Zdef
+    apply ih Zdef.1
+  case arrowl => sorry
+  case eqr => sorry
+  case eql => sorry
+  case appr => sorry
+  case appl => sorry
+  case all A n K j ih =>
+    cases T <;> simp at Zdef
+    case _ K' B =>
+    rcases Zdef with ⟨e1, e2⟩; subst e1 e2
+
+    sorry
+
+theorem FV.zero_not_in_succ {T : Ty} : 0 ∉ T⟨.succ Ty⟩ := by
+  have lem := @FV.var_not_in_one_more (T := T) 0
+  simp at lem; apply lem
+
+theorem FV.subst_congr_var {ℓ1 ℓ2 : List Ty} (σ τ : Subst Ty)
+  (h1 : i < ℓ1.length)
+  (h2 : ℓ1.length = ℓ2.length)
+  : Ty.from_action ((ℓ1.map su ++ σ).act i) = ((ℓ2.map su ++ τ).act i) -> ℓ1[i] = ℓ2[i]
+:= by
+  intro h
+  induction ℓ1 generalizing i ℓ2
+  case _ => simp at h1
+  case _ hd1 tl1 ih =>
+    cases ℓ2; simp at h2
+    case _ hd2 tl2 =>
+      cases i
+      case _ => simp; simp at h; apply h
+      case _ i =>
+        simp at h; simp
+        simp at ih; apply ih _ _ h
+        simp at h2; apply h2
+
+theorem FV.subst_congr_append_get {T : Ty} {ℓ1 ℓ2 : List Ty} {σ τ : Subst Ty}
+  (h1 : i < ℓ1.length)
+  (h2 : ℓ1.length = ℓ2.length)
+  (h3 : i ∈ T)
+  : T[ℓ1.map su ++ σ] = T[ℓ2.map su ++ τ] -> ℓ1[i] = ℓ2[i]
+:= by
+  intro h; induction T generalizing i ℓ1 ℓ2 σ τ
+  case var i =>
+    cases h3; simp at h
+    apply subst_congr_var σ τ h1 h2 h
+  case global => cases h3
+  case arrow A B ih1 ih2 =>
+    simp at h; cases h3
+    case _ h3 => apply ih1 h1 h2 h3 h.1
+    case _ h3 => apply ih2 h1 h2 h3 h.2
+  case all K T ih =>
+    simp at h; cases h3; case _ h3 =>
+    replace ih := @ih (i + 1) (t#0 :: ℓ1⟨.succ Ty⟩) (t#0 :: ℓ2⟨.succ Ty⟩)
+      (σ ∘ Ren.succ Ty) (τ ∘ Ren.succ Ty)
+      (by simp [h1]) (by simp [h2]) h3
+    -- simp at ih; replace ih := ih h
+    -- have lem : (ℓ1⟨Ren.succ Ty⟩[i]'(by grind))⟨Ren.pred Ty⟩ = (ℓ2⟨Ren.succ Ty⟩[i]'(by grind))⟨Ren.pred Ty⟩ := by rw [ih]
+    -- simp at lem
+    sorry
+  case app => sorry
+  case eq => sorry
+
+theorem FV.subst_congr_append {T : Ty} {ℓ1 ℓ2 : List Ty} {σ τ : Subst Ty}
+  (h1 : ∀ i, i < ℓ2.length -> i ∈ T)
+  (h2 : ℓ1.length = ℓ2.length)
+  : T[ℓ1.map su ++ σ] = T[ℓ2.map su ++ τ] -> ℓ1 = ℓ2
+:= by
+  intro h3
+  apply List.ext_get h2
+  intro i q1 q2; simp
+  have lem := h1 i q2
+  apply subst_congr_append_get q1 h2 lem h3
+
+theorem FV.subst_congr_append_lift_get_lemma {T : Ty} {ℓ : List Ty} {σ τ : Subst Ty}
+  : T[ℓ.map su ++ σ] = T[0..ℓ.length ++ τ] -> T[σ.lift ℓ.length] = T[τ.lift ℓ.length]
+:= by
+  sorry
+
+theorem FV.subst_congr_append_append {T : Ty} {ℓ1 ℓ2 ℓ3 : List Ty} {σ τ : Subst Ty}
+  (h1 : ∀ i, i < ℓ2.length -> i + ℓ3.length ∈ T)
+  (h2 : ℓ1.length = ℓ2.length)
+  (h3 : ℓ3.length = k)
+  : T[ℓ3.map su ++ (ℓ1.map su ++ σ)] = T[0..k ++ (ℓ2.map su ++ τ)] -> ℓ1 = ℓ2
+:= by
+  intro h
+  sorry
+-- R[(List.map su As2⟨Ren.add Ty nb⟩.list).reverse ++ (List.map su As1⟨Ren.add Ty nb⟩.list).reverse ++ Subst.add Ty nb] =
+--   R[0..nb ++ ((List.map su As⟨Ren.add Ty nb⟩.list).reverse ++ Subst.add Ty nb)]
+
+end Core
